`DivEquivalence.lean`: add proof obligations for `MOD` opcode

EvmEquivalence/Equivalence/DivEquivalence.lean
@@ -13,6 +13,7 @@ namespace DivOpcodeEquivalence
 inductive arith_op where
   | div
   | sdiv
+  | mod
 
 variable (op : arith_op)
 
@@ -20,10 +21,12 @@ variable (op : arith_op)
 def arith_op.to_binop : arith_op → SortBinStackOp
   | .div  => .DIV_EVM_BinStackOp
   | .sdiv => .SDIV_EVM_BinStackOp
+  | .mod  => .MOD_EVM_BinStackOp
 
 def arith_op.from_k : arith_op → AddSummary.arith_op
  | .div  => .div
  | .sdiv => .sdiv
+ | .mod  => .mod
 
 def divLHS
   {GAS_CELL PC_CELL W0 W1 : SortInt}
@@ -168,6 +171,7 @@ def arith_op.to_defn_Val3 (W0 W1 _Val3 : SortInt) : Prop :=
   match op with
   | .div  => «_/Word__EVM-TYPES_Int_Int_Int» W0 W1 = some _Val3
   | .sdiv => «_/sWord__EVM-TYPES_Int_Int_Int» W0 W1 = some _Val3
+  | .mod  => «_%Word__EVM-TYPES_Int_Int_Int» W0 W1 = some _Val3
 
 theorem rw_addLHS_addRHS
   {GAS_CELL PC_CELL W0 W1 _Val0 _Val3 _Val4 _Val5 _Val6 : SortInt}
@@ -222,6 +226,8 @@ theorem rw_addLHS_addRHS
   . apply (@Rewrites.DIV_SUMMARY_DIV_SUMMARY_USEGAS GAS_CELL PC_CELL W0 W1 _Val0)
     <;> assumption
   . apply (@Rewrites.SDIV_SUMMARY_SDIV_SUMMARY_USEGAS GAS_CELL PC_CELL W0 W1 _Val0)
+    <;> assumption
+  . apply (@Rewrites.MOD_SUMMARY_MOD_SUMMARY_USEGAS GAS_CELL PC_CELL W0 W1 _Val0)
     <;> assumption
 
 theorem div_prestate_equiv
@@ -296,8 +302,9 @@ theorem divWord_divInt_eq (n m : SortInt):
 @[simp]
 def arith_op.do : SortInt → SortInt → SortInt :=
   match op with
-  | .div => (divWord · ·)
+  | .div  => (divWord · ·)
   | .sdiv => (divWord · ·) -- Blatantly wrong
+  | .mod  => (divWord · ·) -- Blatantly wrong
 
 theorem div_poststate_equiv
   {PC_CELL W0 W1 _Val3 _Val4 _Val5 _Val6 : SortInt}
@@ -359,10 +366,15 @@ theorem div_poststate_equiv
     } := by
     cases op
     . -- `div`
-      aesop (add simp [«_-Int_»,«_+Int_», chop'])
-    (add simp [arith_op.to_defn_Val3, divRHS, stateMap, divWord_divInt_eq])
+      aesop (add simp [«_-Int_»,«_+Int_», arith_op.to_defn_Val3, divRHS, stateMap])
+    (add simp [divWord_divInt_eq])
     . -- `sdiv`
       -- To prove this, first `arith_op.do` needs to be fixed for `sdiv`
+      aesop (add simp [«_-Int_»,«_+Int_», arith_op.to_defn_Val3, divRHS, stateMap])
+      sorry
+    . -- `mod`
+      -- To prove this, first `arith_op.do` needs to be fixed for `mod`
+      aesop (add simp [«_-Int_»,«_+Int_», arith_op.to_defn_Val3, divRHS, stateMap])
       sorry
 
 
@@ -372,6 +384,7 @@ def arith_op.gas :=
   match op with
   | .div  => GasConstants.Glow
   | .sdiv => GasConstants.Glow
+  | .mod  => GasConstants.Glow
 
 -- We cannot prove full equivalence for the `EVM.step` function
 -- This is because it doesn't include all semantics such as gas computation
@@ -454,6 +467,9 @@ theorem step_add_equiv
         sorry
       . -- `sdiv`
       -- To prove this, first `arith_op.do` needs to be fixed for `sdiv`
+        sorry
+      .  -- `mod`
+      -- To prove this, first `arith_op.do` needs to be fixed for `mod`
         sorry
 
 attribute [local simp] GasConstants.Glow
@@ -546,6 +562,11 @@ theorem X_add_equiv
       sorry
     . -- `sdiv`
       -- To prove this, first `arith_op.do` needs to be fixed for `sdiv`
+      aesop (add simp [GasInterface.cancun_def, «_-Int_», chop_def, plusInt_def, intMap_add_dist, divLHS, divRHS])
+      (add safe (by rw [intMap_sub_dist])) (add safe (by apply le_of_lt))
+      sorry
+    . -- `mod`
+      -- To prove this, first `arith_op.do` needs to be fixed for `mod`
       aesop (add simp [GasInterface.cancun_def, «_-Int_», chop_def, plusInt_def, intMap_add_dist, divLHS, divRHS])
       (add safe (by rw [intMap_sub_dist])) (add safe (by apply le_of_lt))
       sorry
